one step to prove π₁S₁ = Z

ground_zero/HITs/circle.lean
@@ -58,8 +58,26 @@ namespace circle
   def rec {β : Type u} (b : β) (ℓ : b = b) : S¹ → β :=
   suspension.rec b b (λ _, ℓ)
 
-  theorem recβrule₁ {β : Type u} (b : β) (ℓ : b = b) :
+  def recβrule₁ {β : Type u} (b : β) (ℓ : b = b) :
     rec b ℓ base = b := types.eq.rfl
+
+  def map_functoriality {α : Type u} {β : Type v}
+    {a b c : α} (f : α → β) {p : a = b} {q : b = c} :
+    f # (p ⬝ q) = (f # p) ⬝ (f # q) :=
+  begin induction p, trivial end
+
+  def map_symm {α : Type u} {β : Type v}
+    {a b : α} (f : α → β) {p : a = b} :
+    f # p⁻¹ = (f # p)⁻¹ :=
+  begin induction p, reflexivity end
+
+  def recβrule₂ {β : Type u} (b : β) (ℓ : b = b) :
+    (rec b ℓ # loop) = ℓ := begin
+    transitivity,
+    apply map_functoriality (rec b ℓ),
+    transitivity, apply types.eq.map, apply map_symm,
+    admit
+  end
 
   def ind {β : S¹ → Type u} (b : β base)
     (ℓ : b =[loop] b) : Π (x : S¹), β x :=
@@ -106,75 +124,99 @@ namespace circle
   def three := succ two
   def fourth := succ three
 
+  /-
+    +2 = pos 2
+    +1 = pos 1
+     0 = pos 0
+    −1 = neg 0
+    −2 = neg 1
+  -/
   inductive int
   | pos : ℕ → int
-  | zero
   | neg : ℕ → int
-  /-
-    pos 1 is    2
-    pos 0 is    1
-    zero is     0
-    neg 0 is   −1
-    neg 1 is   −2
-  -/
+
+  instance : has_zero int := ⟨int.pos 0⟩
 
   instance : has_repr int :=
   ⟨λ x, match x with
-  | (int.pos n) := to_string (n + 1)
-  | int.zero := "0"
+  | (int.pos n) := to_string n
   | (int.neg n) := "−" ++ to_string (n + 1)
   end⟩
 
+  def int.auxsucc : ℕ → int
+  | 0 := int.pos 0
+  | (n + 1) := int.neg n
+
   def int.succ : int → int
-  | (int.pos n) := int.pos (n + 1)
-  | int.zero := int.pos 0
-  | (int.neg 0) := int.zero
-  | (int.neg (n + 1)) := int.neg n
+  | (int.neg u) := int.auxsucc u
+  | (int.pos v) := int.pos (v + 1)
+
+  def int.auxpred : ℕ → int
+  | 0 := int.neg 0
+  | (n + 1) := int.pos n
 
   def int.pred : int → int
-  | (int.pos 0) := int.zero
-  | (int.pos (n + 1)) := int.pos n
-  | int.zero := int.neg 0
-  | (int.neg n) := int.neg (n + 1)
+  | (int.neg u) := int.neg (u + 1)
+  | (int.pos v) := int.auxpred v
 
-  theorem int.equiv : int ≃ int := begin
+  def int.equiv : int ≃ int := begin
     existsi int.succ, split; existsi int.pred,
-    { intro n, induction n,
+    repeat {
+      intro n, induction n,
       repeat { trivial },
       { induction n with n ih,
-        repeat { trivial } } },
-    { intro n, induction n,
-      { induction n with n ih,
-        repeat { trivial } },
-      repeat { trivial } }
+        repeat { trivial } }
+    }
   end
 
-  def code : S¹ → Type :=
+  def helix : S¹ → Type :=
   rec int (ua int.equiv)
 
   def pos : ℕ → Ω¹(S¹)
-  | 0 := loop
-  | (n+1) := pos n ⬝ loop
+  | 0 := types.eq.refl base
+  | (n + 1) := pos n ⬝ loop
 
   def neg : ℕ → Ω¹(S¹)
-  | 0 := loop
-  | (n+1) := pos n ⬝ loop⁻¹
-
-  def encode (x : S¹) (p : base = x) : code x :=
-  types.equiv.transport code p int.zero
+  | 0 := loop⁻¹
+  | (n + 1) := pos n ⬝ loop⁻¹
 
   def power : int → Ω¹(S¹)
   | (int.pos n) := pos n
-  | int.zero := idp base
   | (int.neg n) := neg n
 
-  example : power (int.pos 2) = loop ⬝ loop ⬝ loop :=
+  def encode (x : S¹) (p : base = x) : helix x :=
+  types.equiv.transport helix p (int.pos 0)
+
+  example : power (int.pos 2) = loop ⬝ loop :=
   by reflexivity
 
-  abbreviation bicycle : code base → int := id
+  abbreviation bicycle : helix base → int := id
 
   def winding (x : base = base) : int :=
-  bicycle (transport code x int.zero)
+  bicycle (transport helix x $ int.pos 0)
+
+  def transport_characterization
+    {α : Sort u} {β γ : α → Sort v} {a b : α}
+    (f : β a → γ a) (p : a = b) :
+    subst p f = transport γ p ∘ f ∘ transport β p⁻¹ :=
+  begin induction p, reflexivity end
+
+  noncomputable lemma transport_there (x : int) :
+    transport helix loop x = int.succ x := begin
+    transitivity,
+    apply types.equiv.transport_comp id helix loop,
+    transitivity, apply types.equiv.homotopy.eq,
+    apply types.eq.map subst, apply recβrule₂,
+    apply ua.comp_rule
+  end
+
+  def decode : Π (x : S¹), helix x → base = x :=
+  @ind (λ x, helix x → base = x) power (begin
+    apply HITs.interval.funext, intro x,
+    apply types.equiv.homotopy.eq, transitivity,
+    exact transport_characterization power loop,
+    admit
+  end)
 end circle
 
 namespace ncircle
